<?xml version="1.0" encoding="utf-8"?>
<rdf:RDF
   xmlns:dcterms="http://purl.org/dc/terms/"
   xmlns:owl="http://www.w3.org/2002/07/owl#"
   xmlns:rdf="http://www.w3.org/1999/02/22-rdf-syntax-ns#"
   xmlns:rdfs="http://www.w3.org/2000/01/rdf-schema#"
   xmlns:vann="http://purl.org/vocab/vann/"
>
  <rdf:Description rdf:about="https://w3id.org/EVI#usedMLModel">
    <rdf:type rdf:resource="http://www.w3.org/2002/07/owl#ObjectProperty"/>
    <rdfs:subPropertyOf rdf:resource="https://w3id.org/EVI#used"/>
    <rdfs:domain rdf:resource="https://w3id.org/EVI#Computation"/>
    <rdfs:range rdf:resource="https://w3id.org/EVI#MLModel"/>
    <rdfs:comment>The property usedModel is a subproperty of used where domain is Computation and range is MLModel. This is common in fine-tuning or inference tasks.</rdfs:comment>
    <rdfs:label>usedMLModel</rdfs:label>
  </rdf:Description>
  <rdf:Description rdf:about="https://w3id.org/EVI#dataSchema">
    <rdf:type rdf:resource="http://www.w3.org/2002/07/owl#ObjectProperty"/>
    <rdfs:domain rdf:resource="https://w3id.org/EVI#Distribution"/>
    <rdfs:range rdf:resource="https://w3id.org/EVI#Schema"/>
    <rdfs:comment>The dataSchema property describes the content-level schema of a DigitalObject that may be distributed in one or more ways.</rdfs:comment>
    <rdfs:label>dataSchema</rdfs:label>
  </rdf:Description>
  <rdf:Description rdf:nodeID="Nfa1193854ed94c35a7ce1c5dbf50be12">
    <rdf:type rdf:resource="http://www.w3.org/2002/07/owl#Class"/>
    <owl:unionOf rdf:nodeID="Nc43f5969fcee4317bf697e29229e71d8"/>
  </rdf:Description>
  <rdf:Description rdf:about="https://w3id.org/EVI#createdBy">
    <rdf:type rdf:resource="http://www.w3.org/2002/07/owl#ObjectProperty"/>
    <rdfs:subPropertyOf rdf:resource="https://w3id.org/EVI#directlySupportedBy"/>
    <rdfs:domain rdf:resource="https://w3id.org/EVI#DigitalObject"/>
    <rdfs:domain rdf:resource="https://www.w3.org/ns/prov#Entity"/>
    <rdfs:range rdf:resource="https://www.w3.org/ns/prov#Agent"/>
    <rdfs:comment>A prov:Agent is a creator of a prov:Entity if it is createdBy the Agent.</rdfs:comment>
    <rdfs:label>createdBy</rdfs:label>
  </rdf:Description>
  <rdf:Description rdf:about="http://purl.org/vocab/vann/preferredNamespacePrefix">
    <rdf:type rdf:resource="http://www.w3.org/2002/07/owl#AnnotationProperty"/>
  </rdf:Description>
  <rdf:Description rdf:about="http://schema.org/encodingFormat">
    <rdf:type rdf:resource="http://www.w3.org/2002/07/owl#DatatypeProperty"/>
    <rdfs:domain rdf:nodeID="Nfa1193854ed94c35a7ce1c5dbf50be12"/>
    <rdfs:range rdf:resource="http://www.w3.org/2001/XMLSchema#string"/>
    <rdfs:comment>The format of the item in question encoded into.</rdfs:comment>
    <rdfs:label>schema:encodingFormat</rdfs:label>
  </rdf:Description>
  <rdf:Description rdf:about="https://w3id.org/EVI#Package">
    <rdf:type rdf:resource="http://www.w3.org/2002/07/owl#Class"/>
    <rdfs:subClassOf rdf:resource="https://w3id.org/EVI#DigitalObject"/>
    <rdfs:comment>Metadata associated with digital resources that may be packaged together or referenced.</rdfs:comment>
    <rdfs:label>Package</rdfs:label>
  </rdf:Description>
  <rdf:Description rdf:about="http://schema.org/Dataset">
    <rdf:type rdf:resource="http://www.w3.org/2002/07/owl#Class"/>
    <owl:equivalentClass rdf:resource="https://w3id.org/EVI#Dataset"/>
    <rdfs:subClassOf rdf:resource="https://w3id.org/EVI#DigitalObject"/>
    <rdfs:comment>A body of structured information describing some topic(s) of interest.</rdfs:comment>
    <rdfs:label>schema:Dataset</rdfs:label>
  </rdf:Description>
  <rdf:Description rdf:about="https://w3id.org/EVI#modelType">
    <rdf:type rdf:resource="http://www.w3.org/2002/07/owl#DatatypeProperty"/>
    <rdfs:domain rdf:resource="https://w3id.org/EVI#MLModel"/>
    <rdfs:range rdf:resource="http://www.w3.org/2001/XMLSchema#string"/>
    <rdfs:comment>The type or category of the machine learning model (e.g., Classification, Regression, Generative).</rdfs:comment>
    <rdfs:label>modelType</rdfs:label>
  </rdf:Description>
  <rdf:Description rdf:nodeID="Nfb3c47769a3d42419011542893754191">
    <rdf:type rdf:resource="http://www.w3.org/2000/01/rdf-schema#Datatype"/>
    <owl:unionOf rdf:nodeID="N86b379137d3d4f95a9b54f23c7682f1d"/>
  </rdf:Description>
  <rdf:Description rdf:about="http://purl.org/dc/terms/contributor">
    <rdf:type rdf:resource="http://www.w3.org/2002/07/owl#AnnotationProperty"/>
  </rdf:Description>
  <rdf:Description rdf:about="http://schema.org/Service">
    <rdf:type rdf:resource="http://www.w3.org/2002/07/owl#Class"/>
    <owl:equivalentClass rdf:resource="https://w3id.org/EVI#Service"/>
    <rdfs:subClassOf rdf:resource="http://www.w3.org/ns/prov#SoftwareAgent"/>
    <rdfs:comment>A service provided by an organization, e.g. delivery service, print services, etc</rdfs:comment>
    <rdfs:label>schema:Service</rdfs:label>
  </rdf:Description>
  <rdf:Description rdf:about="https://w3id.org/EVI#contentUrl">
    <rdf:type rdf:resource="http://www.w3.org/2002/07/owl#ObjectProperty"/>
    <rdfs:domain rdf:resource="https://w3id.org/EVI#Distribution"/>
    <rdfs:range rdf:resource="https://w3id.org/EVI#DigitalContent"/>
    <rdfs:comment>The contentUrl property provides the access to the actual byes of the DigitalContent that can be downloaded and examined.</rdfs:comment>
    <rdfs:label>contentUrl</rdfs:label>
  </rdf:Description>
  <rdf:Description rdf:about="http://purl.org/dc/terms/title">
    <rdf:type rdf:resource="http://www.w3.org/2002/07/owl#AnnotationProperty"/>
  </rdf:Description>
  <rdf:Description rdf:about="https://w3id.org/EVI#Distribution">
    <rdf:type rdf:resource="http://www.w3.org/2002/07/owl#Class"/>
    <rdfs:subClassOf rdf:resource="https://w3id.org/EVI#DigitalObject"/>
    <rdfs:comment>The placement of instances of DigitalObjects. A single DigitalObject may be represented in multiple forms, hence resulting in multiple distributions. An Image can be encoded and distributed as any of the JPEG, PNG, SVG.</rdfs:comment>
    <rdfs:label>Distribution</rdfs:label>
  </rdf:Description>
  <rdf:Description rdf:about="https://w3id.org/EVI#derivedTo">
    <rdf:type rdf:resource="http://www.w3.org/2002/07/owl#ObjectProperty"/>
    <rdfs:subPropertyOf rdf:resource="https://w3id.org/EVI#directlySupports"/>
    <rdfs:comment>Reverse of derivedFrom property.</rdfs:comment>
    <rdfs:label>derivedTo</rdfs:label>
  </rdf:Description>
  <rdf:Description rdf:about="http://schema.org/SoftwareSourceCode">
    <rdf:type rdf:resource="http://www.w3.org/2002/07/owl#Class"/>
    <owl:equivalentClass rdf:resource="https://w3id.org/EVI#Software"/>
    <rdfs:subClassOf rdf:resource="https://w3id.org/EVI#DigitalObject"/>
    <rdfs:comment>Computer programming source code. Example: Full (compile ready) solutions, code snippet samples, scripts, templates.</rdfs:comment>
    <rdfs:label>schema:SoftwareSourceCode</rdfs:label>
  </rdf:Description>
  <rdf:Description rdf:about="https://w3id.org/EVI#hasBias">
    <rdf:type rdf:resource="http://www.w3.org/2002/07/owl#DatatypeProperty"/>
    <rdfs:domain rdf:resource="https://w3id.org/EVI#MLModel"/>
    <rdfs:range rdf:resource="http://www.w3.org/2001/XMLSchema#string"/>
    <rdfs:comment>Any issue of a model that may consistently deviate its outcome to be incorrect or unfair.</rdfs:comment>
    <rdfs:label>hasBias</rdfs:label>
  </rdf:Description>
  <rdf:Description rdf:about="https://w3id.org/EVI#MLModel">
    <rdf:type rdf:resource="http://www.w3.org/2002/07/owl#Class"/>
    <rdfs:subClassOf rdf:resource="https://w3id.org/EVI#DigitalObject"/>
    <rdfs:comment xml:lang="en">An MLModel is a computational model that has been trained on data to perform a specific task. It is a digital object that captures the learned parameters and architecture resulting from a machine learning training process (Computation).</rdfs:comment>
    <rdfs:label xml:lang="en">MLModel</rdfs:label>
  </rdf:Description>
  <rdf:Description rdf:about="https://www.w3.org/ns/prov#Activity">
    <rdf:type rdf:resource="http://www.w3.org/2002/07/owl#Class"/>
    <rdfs:comment>An Activity is a process by which an Entity is produced, modified, consumed or used.</rdfs:comment>
    <rdfs:label>prov:Activity</rdfs:label>
  </rdf:Description>
  <rdf:Description rdf:about="https://w3id.org/EVI#indirectlyChallengedBy">
    <rdf:type rdf:resource="http://www.w3.org/2002/07/owl#ObjectProperty"/>
    <rdfs:subPropertyOf rdf:resource="https://w3id.org/EVI#challengedBy"/>
    <owl:inverseOf rdf:resource="https://w3id.org/EVI#indirectlyChallenges"/>
    <rdfs:comment>Reverse of indirectlyChallenges property.</rdfs:comment>
    <rdfs:label>indirectlyChallengedBy</rdfs:label>
  </rdf:Description>
  <rdf:Description rdf:about="http://www.w3.org/ns/prov#SoftwareAgent">
    <rdf:type rdf:resource="http://www.w3.org/2002/07/owl#Class"/>
    <rdfs:subClassOf rdf:resource="https://www.w3.org/ns/prov#Agent"/>
    <rdfs:comment>A Service is considered a SoftwareAgent that can be invoked and executed. A Software is different from SoftwareAgent in the context that it can be downloaded.</rdfs:comment>
    <rdfs:label>prov:SoftwareAgent</rdfs:label>
  </rdf:Description>
  <rdf:Description rdf:about="http://www.w3.org/ns/prov#Bundle">
    <rdf:type rdf:resource="http://www.w3.org/2002/07/owl#Class"/>
    <rdfs:comment>A bundle is a named set of provenance descriptions, and is itself an Entity, so allowing provenance of provenance to be expressed.</rdfs:comment>
    <rdfs:label>prov:Bundle</rdfs:label>
  </rdf:Description>
  <rdf:Description rdf:about="https://w3id.org/EVI#Method">
    <rdf:type rdf:resource="http://www.w3.org/2002/07/owl#Class"/>
    <rdfs:subClassOf rdf:resource="https://w3id.org/EVI#DigitalObject"/>
    <rdfs:comment>A descriptive recipe describing how a Representation is made or obtained. It describes an Activity, and may referTo some Material as a component of the recipe.</rdfs:comment>
    <rdfs:label>Method</rdfs:label>
  </rdf:Description>
  <rdf:Description rdf:about="https://w3id.org/EVI#indirectlyChallenges">
    <rdf:type rdf:resource="http://www.w3.org/2002/07/owl#ObjectProperty"/>
    <rdfs:subPropertyOf rdf:resource="https://w3id.org/EVI#challenges"/>
    <rdfs:domain rdf:resource="https://w3id.org/EVI#DigitalObject"/>
    <rdfs:range rdf:resource="https://w3id.org/EVI#DigitalObject"/>
    <owl:propertyChainAxiom rdf:nodeID="N2a95c47191824e0a8d53674395752438"/>
    <rdfs:comment>The indirectlyChallenges property establishes a relation between instances of DigitalObjects when one indirectly challenges the other entailed by property chaining.</rdfs:comment>
    <rdfs:label>indirectlyChallenges</rdfs:label>
  </rdf:Description>
  <rdf:Description rdf:about="https://w3id.org/EVI#distributedFrom">
    <rdf:type rdf:resource="http://www.w3.org/2002/07/owl#ObjectProperty"/>
    <owl:inverseOf rdf:resource="https://w3id.org/EVI#hasDistribution"/>
    <rdfs:comment>Reverse of hasDistribution property.</rdfs:comment>
    <rdfs:label>distributedFrom</rdfs:label>
  </rdf:Description>
  <rdf:Description rdf:about="https://w3id.org/EVI#inputSize">
    <rdf:type rdf:resource="http://www.w3.org/2002/07/owl#DatatypeProperty"/>
    <rdfs:domain rdf:resource="https://w3id.org/EVI#MLModel"/>
    <rdfs:range rdf:resource="http://www.w3.org/2001/XMLSchema#string"/>
    <rdfs:comment>The expected input size or shape the model is designed to receive and process at one time. For example, image classificatoin models such as ResNet, VGG commonly use 224x224 pixels with 3 channels while Language Models such as BERT, GPT use tokens or context length from thousand to millions.</rdfs:comment>
    <rdfs:label>inputSize</rdfs:label>
  </rdf:Description>
  <rdf:Description rdf:about="http://purl.org/dc/terms/creator">
    <rdf:type rdf:resource="http://www.w3.org/2002/07/owl#AnnotationProperty"/>
    <rdf:type rdf:resource="http://www.w3.org/2002/07/owl#ObjectProperty"/>
    <rdfs:range rdf:resource="https://www.w3.org/ns/prov#Agent"/>
    <rdfs:domain rdf:resource="https://w3id.org/EVI#DigitalObject"/>
    <rdfs:comment>An entity responsible for making the resource. Examples of a creator include a person, an organization, or a service i.e. a SoftwareAgent. Typically, the name of a creator should be used to indicate the entity.</rdfs:comment>
    <rdfs:label>terms:creator</rdfs:label>
  </rdf:Description>
  <rdf:Description rdf:about="https://w3id.org/EVI#usedService">
    <rdf:type rdf:resource="http://www.w3.org/2002/07/owl#ObjectProperty"/>
    <rdfs:subPropertyOf rdf:resource="https://w3id.org/EVI#used"/>
    <rdfs:domain rdf:resource="https://w3id.org/EVI#Computation"/>
    <rdfs:range rdf:resource="https://w3id.org/EVI#Service"/>
    <rdfs:comment>The property usedService is a subproperty of used where domain is Computation and range is Service.</rdfs:comment>
    <rdfs:label>usedService</rdfs:label>
  </rdf:Description>
  <rdf:Description rdf:about="https://w3id.org/EVI#Dataset">
    <rdf:type rdf:resource="http://www.w3.org/2002/07/owl#Class"/>
    <rdfs:subClassOf rdf:resource="https://w3id.org/EVI#DigitalObject"/>
    <rdfs:comment>A body of structured information describing some topic(s) of interest.</rdfs:comment>
    <rdfs:label>Dataset</rdfs:label>
  </rdf:Description>
  <rdf:Description rdf:about="https://w3id.org/EVI#parametersCount">
    <rdf:type rdf:resource="http://www.w3.org/2002/07/owl#DatatypeProperty"/>
    <rdfs:domain rdf:resource="https://w3id.org/EVI#MLModel"/>
    <rdfs:range rdf:resource="http://www.w3.org/2001/XMLSchema#string"/>
    <rdfs:comment>The number of variables a model learns during training. For current LLM models, this number ranges from millions to trillions that determines the performance and complexity of these models.</rdfs:comment>
    <rdfs:label>parametersCount</rdfs:label>
  </rdf:Description>
  <rdf:Description rdf:about="https://w3id.org/EVI#EvidenceGraph">
    <rdf:type rdf:resource="http://www.w3.org/2002/07/owl#Class"/>
    <rdfs:subClassOf rdf:resource="https://w3id.org/EVI#DigitalObject"/>
    <rdfs:comment>An EvidenceGraph is a directed acyclic graph

Ev = (Rn, r+, r-)

where Rn is a set of Representations, r+ ∈ RnXRn is a set of supports relations, r- ∈ RnXRn is a set of challenge relations, and R+∩R- = Φ.

EvidenceGraphs are bipolar argumentation frameworks (Cayrol &amp;amp; Lagasquie-Schiex, 2009) represented as RDF named graphs.</rdfs:comment>
    <rdfs:label>EvidenceGraph</rdfs:label>
  </rdf:Description>
  <rdf:Description rdf:about="https://w3id.org/EVI#created">
    <rdf:type rdf:resource="http://www.w3.org/2002/07/owl#ObjectProperty"/>
    <rdfs:subPropertyOf rdf:resource="https://w3id.org/EVI#directlySupports"/>
    <owl:inverseOf rdf:resource="https://w3id.org/EVI#createdBy"/>
    <rdfs:comment>Reverse of createdBy property.</rdfs:comment>
    <rdfs:label>created</rdfs:label>
  </rdf:Description>
  <rdf:Description rdf:about="https://w3id.org/EVI#generated">
    <rdf:type rdf:resource="http://www.w3.org/2002/07/owl#ObjectProperty"/>
    <rdfs:subPropertyOf rdf:resource="https://w3id.org/EVI#directlySupports"/>
    <owl:inverseOf rdf:resource="https://w3id.org/EVI#generatedBy"/>
    <rdfs:comment>Reverse of generatedBy property.</rdfs:comment>
    <rdfs:label>generated</rdfs:label>
  </rdf:Description>
  <rdf:Description rdf:about="https://w3id.org/EVI#Claim">
    <rdf:type rdf:resource="http://www.w3.org/2002/07/owl#Class"/>
    <rdfs:subClassOf rdf:resource="https://w3id.org/EVI#DigitalObject"/>
    <rdfs:comment>A Claim is a declarative sentence or assertion. Claims are defeasible.</rdfs:comment>
    <rdfs:label>Claim</rdfs:label>
  </rdf:Description>
  <rdf:Description rdf:about="https://w3id.org/EVI">
    <rdf:type rdf:resource="http://www.w3.org/2002/07/owl#Ontology"/>
    <rdf:type rdf:resource="http://www.w3.org/2002/07/owl#NamedIndividual"/>
    <owl:versionIRI rdf:resource="https://w3id.org/EVI/1.2"/>
    <owl:versionIRI xml:lang="en">http://www.w3.org/2002/07/owl</owl:versionIRI>
    <dcterms:contributor rdf:resource="https://github.com/jniestroy"/>
    <dcterms:contributor rdf:resource="https://github.com/mlev71"/>
    <dcterms:created xml:lang="en">2020-07-27</dcterms:created>
    <dcterms:description xml:lang="en">The Evidence Graph ontology extends core concepts from the W3C Provenance Ontology PROV-O and Bioschemas' Profiles to describe evidence for correctness of findings in biomedical publications. The semantic data model in EVI is expressed using OWL2 Web Ontology Language (OWL2).</dcterms:description>
    <dcterms:license rdf:resource="http://creativecommons.org/licenses/by-nc-sa/2.0/"/>
    <dcterms:modified xml:lang="en">2025-11-07</dcterms:modified>
    <dcterms:title xml:lang="en">EVI: Evidence Graph Ontology</dcterms:title>
    <vann:preferredNamespacePrefix>evi</vann:preferredNamespacePrefix>
    <vann:preferredNamespaceUri rdf:resource="http://w3id.org/EVI"/>
    <owl:priorVersion xml:lang="en">1.1</owl:priorVersion>
    <owl:versionInfo xml:lang="en">1.2</owl:versionInfo>
    <dcterms:creator rdf:resource="https://orcid.org/0000-0003-4060-7360"/>
    <dcterms:creator rdf:resource="https://orcid.org/0000-0003-4647-3877"/>
  </rdf:Description>
  <rdf:Description rdf:about="https://w3id.org/EVI#directlySupportedBy">
    <rdf:type rdf:resource="http://www.w3.org/2002/07/owl#ObjectProperty"/>
    <rdfs:subPropertyOf rdf:resource="https://w3id.org/EVI#supportedBy"/>
    <owl:inverseOf rdf:resource="https://w3id.org/EVI#directlySupports"/>
    <rdfs:comment>The use of directlySupportedBy property is intended to establish a direct relation between instances of DigitalObjects.</rdfs:comment>
    <rdfs:label>directlySupportedBy</rdfs:label>
  </rdf:Description>
  <rdf:Description rdf:nodeID="Nce33bcf0eca3438ca339c18cbafc8472">
    <rdf:first rdf:resource="http://www.w3.org/2001/XMLSchema#anyURI"/>
    <rdf:rest rdf:nodeID="N3d13ed0d04f04c51a095f813997f2c7e"/>
  </rdf:Description>
  <rdf:Description rdf:about="https://w3id.org/EVI#additionalDocumentation">
    <rdf:type rdf:resource="http://www.w3.org/2002/07/owl#DatatypeProperty"/>
    <rdfs:domain rdf:nodeID="N5c9c66fc760d4252ad7a42ce375a8b4e"/>
    <rdfs:range rdf:nodeID="N2419b5b626154ae6b71f75b474dc6817"/>
    <rdfs:comment>Any additional information of the item that may be useful.</rdfs:comment>
    <rdfs:label>additionalDocumentation</rdfs:label>
  </rdf:Description>
  <rdf:Description rdf:about="https://w3id.org/EVI#directlyChallenges">
    <rdf:type rdf:resource="http://www.w3.org/2002/07/owl#ObjectProperty"/>
    <rdfs:subPropertyOf rdf:resource="https://w3id.org/EVI#challenges"/>
    <rdfs:domain rdf:resource="https://w3id.org/EVI#DigitalObject"/>
    <rdfs:range rdf:resource="https://w3id.org/EVI#DigitalObject"/>
    <rdfs:comment>The directlyChallenges property establishes a relation between instances of DigitalObjects A and B when A asserts that B is wrong or deficient. It is non-transitive, entailing indirectlyChallenges properties on DigitalObjects supportedBy the DigitalObject it directlyChallenges, via a property chain rule.</rdfs:comment>
    <rdfs:label>directlyChallenges</rdfs:label>
  </rdf:Description>
  <rdf:Description rdf:about="https://w3id.org/EVI#usedDataset">
    <rdf:type rdf:resource="http://www.w3.org/2002/07/owl#ObjectProperty"/>
    <rdfs:subPropertyOf rdf:resource="https://w3id.org/EVI#used"/>
    <rdfs:domain rdf:resource="https://w3id.org/EVI#Computation"/>
    <rdfs:range rdf:resource="https://w3id.org/EVI#Dataset"/>
    <rdfs:comment>The property usedDataset is a subproperty of used where domain is Computation and range is Dataset.</rdfs:comment>
    <rdfs:label>usedDataset</rdfs:label>
  </rdf:Description>
  <rdf:Description rdf:about="https://w3id.org/EVI#directlySupports">
    <rdf:type rdf:resource="http://www.w3.org/2002/07/owl#ObjectProperty"/>
    <rdfs:subPropertyOf rdf:resource="https://w3id.org/EVI#supports"/>
    <rdfs:comment>The directlySupports property is a non-transitive version of supports, a subproperty of supports. directlySupports is a superproperty of the properties attributed (inverse of attributedTo), derived (inverse of derivedFrom), associated (inverse of associatedWith), used, and generated (inverse of generatedBy).</rdfs:comment>
    <rdfs:label>directlySupports</rdfs:label>
  </rdf:Description>
  <rdf:Description rdf:about="http://schema.org/startTime">
    <rdf:type rdf:resource="http://www.w3.org/2002/07/owl#DatatypeProperty"/>
    <rdfs:domain rdf:resource="https://w3id.org/EVI#Computation"/>
    <rdfs:range rdf:resource="http://www.w3.org/2001/XMLSchema#dateTime"/>
    <rdfs:comment>The startTime of something. For a reserved event or service (e.g. FoodEstablishmentReservation), the time that it is expected to start. For actions that span a period of time, when the action was performed. e.g. John wrote a book from January to December. For media, including audio and video, it's the time offset of the start of a clip within a larger file.

Note that Event uses startDate/endDate instead of startTime/endTime, even when describing dates with times. This situation may be clarified in future revisions.</rdfs:comment>
    <rdfs:label>schema:startTime</rdfs:label>
  </rdf:Description>
  <rdf:Description rdf:about="https://w3id.org/EVI#Image">
    <rdf:type rdf:resource="http://www.w3.org/2002/07/owl#Class"/>
    <rdfs:subClassOf rdf:resource="https://w3id.org/EVI#Dataset"/>
    <rdfs:comment>An Image is a visual representation of structured or unstructured data produced digitally.</rdfs:comment>
    <rdfs:label>Image</rdfs:label>
  </rdf:Description>
  <rdf:Description rdf:about="https://w3id.org/EVI#supports">
    <rdf:type rdf:resource="http://www.w3.org/2002/07/owl#ObjectProperty"/>
    <rdf:type rdf:resource="http://www.w3.org/2002/07/owl#TransitiveProperty"/>
    <rdfs:domain rdf:resource="https://w3id.org/EVI#DigitalObject"/>
    <rdfs:range rdf:resource="https://w3id.org/EVI#DigitalObject"/>
    <rdfs:comment>The supports property is a transitive relation between DigitalObjects entailed by its subproperty, directlySupports, which is non-transitive. In EvidenceGraphs, if A supports B, then the correctness (truth value) of A provides a warrant for belief in the correctness (truth value) of B.</rdfs:comment>
    <rdfs:label>supports</rdfs:label>
  </rdf:Description>
  <rdf:Description rdf:about="http://schema.org/datePublished">
    <rdf:type rdf:resource="http://www.w3.org/2002/07/owl#DatatypeProperty"/>
    <rdfs:domain rdf:nodeID="Na341cade5df7416fa0fc8cd5e200d20a"/>
    <rdfs:range rdf:resource="http://www.w3.org/2001/XMLSchema#dateTime"/>
    <rdfs:comment>Date when the item was first published.</rdfs:comment>
    <rdfs:label>schema:datePublished</rdfs:label>
  </rdf:Description>
  <rdf:Description rdf:about="https://w3id.org/EVI#associatedPublication">
    <rdf:type rdf:resource="http://www.w3.org/2002/07/owl#DatatypeProperty"/>
    <rdfs:domain rdf:nodeID="N656d1f893b73479faf005b0166bb7695"/>
    <rdfs:range rdf:nodeID="Nfb3c47769a3d42419011542893754191"/>
    <rdfs:comment>Refenrece to the publications where the item or its relevant information can be discovered.</rdfs:comment>
    <rdfs:label>associatedPublication</rdfs:label>
  </rdf:Description>
  <rdf:Description rdf:about="https://w3id.org/EVI#supportedBy">
    <rdf:type rdf:resource="http://www.w3.org/2002/07/owl#ObjectProperty"/>
    <owl:inverseOf rdf:resource="https://w3id.org/EVI#supports"/>
    <rdfs:comment>The supportedBy property is a transitive relation between DigitalObjects.</rdfs:comment>
    <rdfs:label>supportedBy</rdfs:label>
  </rdf:Description>
  <rdf:Description rdf:about="https://w3id.org/EVI#mlModelUsedBy">
    <rdf:type rdf:resource="http://www.w3.org/2002/07/owl#ObjectProperty"/>
    <rdfs:subPropertyOf rdf:resource="https://w3id.org/EVI#usedBy"/>
    <owl:inverseOf rdf:resource="https://w3id.org/EVI#usedMLModel"/>
    <rdfs:comment>Reverse of usedMLModel property.</rdfs:comment>
    <rdfs:label>mlModelUsedBy</rdfs:label>
  </rdf:Description>
  <rdf:Description rdf:about="http://schema.org/identifier">
    <rdf:type rdf:resource="http://www.w3.org/2002/07/owl#DatatypeProperty"/>
    <rdfs:range rdf:resource="http://www.w3.org/2001/XMLSchema#anyURI"/>
    <rdfs:comment>The identifier property represents any kind of identifier for any kind of Thing, such as ISBNs, GTIN codes, UUIDs etc. Schema.org provides dedicated properties for representing many of these, either as textual strings or as URL (URI) links.</rdfs:comment>
    <rdfs:label>schema:identifier</rdfs:label>
  </rdf:Description>
  <rdf:Description rdf:about="https://w3id.org/EVI#associateFor">
    <rdf:type rdf:resource="http://www.w3.org/2002/07/owl#ObjectProperty"/>
    <rdfs:subPropertyOf rdf:resource="https://w3id.org/EVI#directlySupports"/>
    <owl:inverseOf rdf:resource="https://w3id.org/EVI#associatedWith"/>
    <rdfs:comment>Reverse of associatedWith property.</rdfs:comment>
    <rdfs:label>associateFor</rdfs:label>
  </rdf:Description>
  <rdf:Description rdf:about="https://w3id.org/EVI#modelFormat">
    <rdf:type rdf:resource="http://www.w3.org/2002/07/owl#DatatypeProperty"/>
    <rdfs:domain rdf:resource="https://w3id.org/EVI#MLModel"/>
    <rdfs:range rdf:resource="http://www.w3.org/2001/XMLSchema#string"/>
    <rdfs:comment>The file format of the model (e.g., ONNX, HDF5, Pickle).</rdfs:comment>
    <rdfs:label>modelFormat</rdfs:label>
  </rdf:Description>
  <rdf:Description rdf:about="http://schema.org/Organization">
    <rdf:type rdf:resource="http://www.w3.org/2002/07/owl#Class"/>
    <owl:equivalentClass rdf:resource="https://www.w3.org/ns/prov#Organization"/>
    <rdfs:subClassOf rdf:resource="https://www.w3.org/ns/prov#Agent"/>
    <rdfs:comment>An organization such as a school, NGO, corporation, club, etc.</rdfs:comment>
    <rdfs:label>schema:Organization</rdfs:label>
  </rdf:Description>
  <rdf:Description rdf:about="https://w3id.org/EVI#Computation">
    <rdf:type rdf:resource="http://www.w3.org/2002/07/owl#Class"/>
    <rdfs:subClassOf rdf:resource="https://www.w3.org/ns/prov#Activity"/>
    <rdfs:comment>Computation is an Activity performed on a Dataset with the help of a Software.</rdfs:comment>
    <rdfs:label>Computation</rdfs:label>
  </rdf:Description>
  <rdf:Description rdf:nodeID="N2b0e6260a6d14db3b35eca0c82c66508">
    <rdf:first rdf:resource="https://w3id.org/EVI#supports"/>
    <rdf:rest rdf:resource="http://www.w3.org/1999/02/22-rdf-syntax-ns#nil"/>
  </rdf:Description>
  <rdf:Description rdf:about="https://www.w3.org/ns/prov#Organization">
    <rdf:type rdf:resource="http://www.w3.org/2002/07/owl#Class"/>
    <rdfs:subClassOf rdf:resource="https://www.w3.org/ns/prov#Agent"/>
    <rdfs:comment>An Organization is a social or legal institution with structure and purpose such as a company, society, university, sports team, etc.</rdfs:comment>
    <rdfs:label>prov:Organization</rdfs:label>
  </rdf:Description>
  <rdf:Description rdf:about="https://w3id.org/EVI#packages">
    <rdf:type rdf:resource="http://www.w3.org/2002/07/owl#ObjectProperty"/>
    <rdfs:domain rdf:resource="https://w3id.org/EVI#Container"/>
    <rdfs:range rdf:resource="https://w3id.org/EVI#Software"/>
    <rdfs:comment>Instances of software can be packaged by the instances of containers.</rdfs:comment>
    <rdfs:label>packages</rdfs:label>
  </rdf:Description>
  <rdf:Description rdf:about="https://w3id.org/EVI#contains">
    <rdf:type rdf:resource="http://www.w3.org/2002/07/owl#ObjectProperty"/>
    <rdf:type rdf:resource="http://www.w3.org/2002/07/owl#TransitiveProperty"/>
    <rdfs:domain rdf:resource="https://w3id.org/EVI#DigitalObject"/>
    <rdfs:range rdf:resource="https://w3id.org/EVI#DigitalObject"/>
    <rdfs:comment>Instances of DigitalObjects may contain instances of other DigitalObjects.</rdfs:comment>
    <rdfs:label>contains</rdfs:label>
  </rdf:Description>
  <rdf:Description rdf:nodeID="N30ab2c1a589242efaa464bbd4a9d22f5">
    <rdf:first rdf:resource="https://w3id.org/EVI#Computation"/>
    <rdf:rest rdf:nodeID="Nb3b2a52811b1478d8a737df63710616d"/>
  </rdf:Description>
  <rdf:Description rdf:nodeID="N37ffb79d9a2d409c92e86008f6519fed">
    <rdf:first rdf:resource="https://w3id.org/EVI#Dataset"/>
    <rdf:rest rdf:nodeID="N7ac8284c91ac4bffa957425012b54369"/>
  </rdf:Description>
  <rdf:Description rdf:about="https://w3id.org/EVI#Service">
    <rdf:type rdf:resource="http://www.w3.org/2002/07/owl#Class"/>
    <rdfs:subClassOf rdf:resource="http://www.w3.org/ns/prov#SoftwareAgent"/>
    <rdfs:comment>A Service is an Activity accessed online, which executes a Computation.</rdfs:comment>
    <rdfs:label>Service</rdfs:label>
  </rdf:Description>
  <rdf:Description rdf:about="https://w3id.org/EVI#Reference">
    <rdf:type rdf:resource="http://www.w3.org/2002/07/owl#Class"/>
    <rdfs:subClassOf rdf:resource="https://w3id.org/EVI#DigitalObject"/>
    <rdfs:comment>A Reference is a bibliographic record. References are Representations which represent and attribute archived digital or bibliographic objects, including Articles, Datasets, and Software.</rdfs:comment>
    <rdfs:label>Reference</rdfs:label>
  </rdf:Description>
  <rdf:Description rdf:about="http://schema.org/license">
    <rdf:type rdf:resource="http://www.w3.org/2002/07/owl#DatatypeProperty"/>
    <rdfs:domain rdf:nodeID="Nee56742a1c524eefba7f015572ab5965"/>
    <rdfs:range rdf:nodeID="N640fb088466a41e683040b8b91eceb73"/>
    <rdfs:comment>A license document that applies to this content, typically indicated by URL.</rdfs:comment>
    <rdfs:label>schema:license</rdfs:label>
  </rdf:Description>
  <rdf:Description rdf:about="https://www.w3.org/ns/prov#Person">
    <rdf:type rdf:resource="http://www.w3.org/2002/07/owl#Class"/>
    <rdfs:subClassOf rdf:resource="https://www.w3.org/ns/prov#Agent"/>
    <rdfs:comment>A Person is a human Agent.</rdfs:comment>
    <rdfs:label>prov:Person</rdfs:label>
  </rdf:Description>
  <rdf:Description rdf:about="http://schema.org/name">
    <rdf:type rdf:resource="http://www.w3.org/2002/07/owl#DatatypeProperty"/>
    <rdfs:domain rdf:resource="http://www.w3.org/2002/07/owl#Thing"/>
    <rdfs:range rdf:resource="http://www.w3.org/2001/XMLSchema#string"/>
    <rdfs:comment>The name of the item.</rdfs:comment>
    <rdfs:label>schema:name</rdfs:label>
  </rdf:Description>
  <rdf:Description rdf:nodeID="N889afee0109c4667a285af07340dad3c">
    <rdf:first rdf:resource="https://w3id.org/EVI#Computation"/>
    <rdf:rest rdf:nodeID="N8f59881000c34ea888a66d16e3fcc7a7"/>
  </rdf:Description>
  <rdf:Description rdf:nodeID="Nd1e9f5743eed4ccea29525833a324206">
    <rdf:first rdf:resource="https://w3id.org/EVI#Dataset"/>
    <rdf:rest rdf:nodeID="N666773303e1446038816e54e3e21f79c"/>
  </rdf:Description>
  <rdf:Description rdf:about="https://w3id.org/EVI#challengedBy">
    <rdf:type rdf:resource="http://www.w3.org/2002/07/owl#ObjectProperty"/>
    <owl:inverseOf rdf:resource="https://w3id.org/EVI#challenges"/>
    <rdfs:comment>Reverse of challenges property.</rdfs:comment>
    <rdfs:label>challengedBy</rdfs:label>
  </rdf:Description>
  <rdf:Description rdf:nodeID="N1a0acc0547f2406aa0bf383c1955b46f">
    <rdf:type rdf:resource="http://www.w3.org/2002/07/owl#Class"/>
    <owl:unionOf rdf:nodeID="N3819eb89e8d84d5c8bd27601f1b80a00"/>
  </rdf:Description>
  <rdf:Description rdf:about="http://schema.org/Article">
    <rdf:type rdf:resource="http://www.w3.org/2002/07/owl#Class"/>
    <owl:equivalentClass rdf:resource="https://w3id.org/EVI#Article"/>
    <rdfs:subClassOf rdf:resource="https://w3id.org/EVI#DigitalObject"/>
    <rdfs:comment>An article, such as a news article or piece of investigative report. Newspapers and magazines have articles of many different types and this is intended to cover them all.</rdfs:comment>
    <rdfs:label>schema:Article</rdfs:label>
  </rdf:Description>
  <rdf:Description rdf:nodeID="N4172f5b5abb849a998fabbdaea104bde">
    <rdf:first rdf:resource="http://www.w3.org/2001/XMLSchema#string"/>
    <rdf:rest rdf:resource="http://www.w3.org/1999/02/22-rdf-syntax-ns#nil"/>
  </rdf:Description>
  <rdf:Description rdf:about="https://w3id.org/EVI#describes">
    <rdf:type rdf:resource="http://www.w3.org/2002/07/owl#ObjectProperty"/>
    <rdfs:domain rdf:resource="https://w3id.org/EVI#Method"/>
    <rdfs:range rdf:resource="https://www.w3.org/ns/prov#Activity"/>
    <rdfs:comment>The describes property is used when a Method, generally composed with a block of text, narrates a prov:Activity that takes place.</rdfs:comment>
    <rdfs:label>describes</rdfs:label>
  </rdf:Description>
  <rdf:Description rdf:about="https://orcid.org/0000-0003-4060-7360">
    <rdf:type rdf:resource="http://www.w3.org/2002/07/owl#NamedIndividual"/>
  </rdf:Description>
  <rdf:Description rdf:about="http://schema.org/SoftwareApplication">
    <rdf:type rdf:resource="http://www.w3.org/2002/07/owl#Class"/>
    <owl:equivalentClass rdf:resource="https://w3id.org/EVI#Software"/>
    <rdfs:subClassOf rdf:resource="https://w3id.org/EVI#DigitalObject"/>
    <rdfs:comment>A software application.</rdfs:comment>
    <rdfs:label>schema:SoftwareApplication</rdfs:label>
  </rdf:Description>
  <rdf:Description rdf:about="https://w3id.org/EVI#publicationVenue">
    <rdf:type rdf:resource="http://www.w3.org/2002/07/owl#DatatypeProperty"/>
    <rdfs:domain rdf:nodeID="N69e9bc263b7a492da24c709fe879c29c"/>
    <rdfs:range rdf:resource="http://www.w3.org/2001/XMLSchema#string"/>
    <rdfs:comment>The (digital/physical) name where the item was published.</rdfs:comment>
    <rdfs:label>publicationVenue</rdfs:label>
  </rdf:Description>
  <rdf:Description rdf:about="https://w3id.org/EVI#Software">
    <rdf:type rdf:resource="http://www.w3.org/2002/07/owl#Class"/>
    <rdfs:subClassOf rdf:resource="https://w3id.org/EVI#DigitalObject"/>
    <rdfs:comment>Software is a specific set of computer-interpretable instructions to perform one or more Computations.</rdfs:comment>
    <rdfs:label>Software</rdfs:label>
  </rdf:Description>
  <rdf:Description rdf:about="http://schema.org/keywords">
    <rdf:type rdf:resource="http://www.w3.org/2002/07/owl#DatatypeProperty"/>
    <rdfs:domain rdf:nodeID="Nba3cc71b22eb418c8b03f631e364a8d4"/>
    <rdfs:range rdf:resource="http://www.w3.org/2001/XMLSchema#string"/>
    <rdfs:comment>Keywords or tags used to describe some item. Multiple textual entries in a keywords list are typically delimited by commas, or by repeating the property.</rdfs:comment>
    <rdfs:label>schema:keywords</rdfs:label>
  </rdf:Description>
  <rdf:Description rdf:nodeID="Nddeb8932f5be4be1b2be7c3b08c3cd83">
    <rdf:first rdf:resource="https://w3id.org/EVI#Software"/>
    <rdf:rest rdf:resource="http://www.w3.org/1999/02/22-rdf-syntax-ns#nil"/>
  </rdf:Description>
  <rdf:Description rdf:nodeID="N5301cd9a878d4955a4aeb3665dd0063a">
    <rdf:first rdf:resource="https://w3id.org/EVI#Computation"/>
    <rdf:rest rdf:nodeID="N4eddae4666c74b9c97a49ca0b2b38b20"/>
  </rdf:Description>
  <rdf:Description rdf:about="https://w3id.org/EVI#representedBy">
    <rdf:type rdf:resource="http://www.w3.org/2002/07/owl#ObjectProperty"/>
    <owl:inverseOf rdf:resource="https://w3id.org/EVI#represents"/>
    <rdfs:comment>Reverse of represents property.</rdfs:comment>
    <rdfs:label>representedBy</rdfs:label>
  </rdf:Description>
  <rdf:Description rdf:about="https://w3id.org/EVI#state">
    <rdf:type rdf:resource="http://www.w3.org/2002/07/owl#DatatypeProperty"/>
    <rdfs:domain rdf:resource="https://w3id.org/EVI#Claim"/>
    <rdfs:range rdf:resource="http://www.w3.org/2001/XMLSchema#string"/>
    <rdfs:comment>Textual representation of a claim</rdfs:comment>
    <rdfs:label>state</rdfs:label>
  </rdf:Description>
  <rdf:Description rdf:about="http://purl.org/dc/terms/created">
    <rdf:type rdf:resource="http://www.w3.org/2002/07/owl#AnnotationProperty"/>
  </rdf:Description>
  <rdf:Description rdf:about="https://w3id.org/EVI#used">
    <rdf:type rdf:resource="http://www.w3.org/2002/07/owl#ObjectProperty"/>
    <rdfs:subPropertyOf rdf:resource="https://w3id.org/EVI#directlySupportedBy"/>
    <owl:inverseOf rdf:resource="https://w3id.org/EVI#usedBy"/>
    <rdfs:domain rdf:resource="https://www.w3.org/ns/prov#Activity"/>
    <rdfs:range rdf:resource="https://www.w3.org/ns/prov#Entity"/>
    <rdfs:comment>An Activity used an Entity, when the Entity (such as a Dataset or a Software) was instrumental in enabling that Activity to occur.</rdfs:comment>
    <rdfs:label>used</rdfs:label>
  </rdf:Description>
  <rdf:Description rdf:nodeID="N3819eb89e8d84d5c8bd27601f1b80a00">
    <rdf:first rdf:resource="https://w3id.org/EVI#Dataset"/>
    <rdf:rest rdf:nodeID="N9fe00874ee1140099f4ff5d1a8a06bd2"/>
  </rdf:Description>
  <rdf:Description rdf:about="https://w3id.org/EVI#Container">
    <rdf:type rdf:resource="http://www.w3.org/2002/07/owl#Class"/>
    <rdfs:subClassOf rdf:resource="https://w3id.org/EVI#DigitalObject"/>
    <rdfs:comment>A container is a digital object that can be defined as packages of software. Instances of containers are accompanied by all necessary dependencies such as specific versions, runtime environment and required libraries for execution.</rdfs:comment>
    <rdfs:label>Container</rdfs:label>
  </rdf:Description>
  <rdf:Description rdf:about="http://schema.org/Claim">
    <rdf:type rdf:resource="http://www.w3.org/2002/07/owl#Class"/>
    <owl:equivalentClass rdf:resource="https://w3id.org/EVI#Claim"/>
    <rdfs:subClassOf rdf:resource="https://w3id.org/EVI#DigitalObject"/>
    <rdfs:comment>A Claim in Schema.org represents a specific, factually-oriented claim that could be the itemReviewed in a ClaimReview. The content of a claim can be summarized with the text property. Variations on well known claims can have their common identity indicated via sameAs links, and summarized with a name. Ideally, a Claim description includes enough contextual information to minimize the risk of ambiguity or inclarity. In practice, many claims are better understood in the context in which they appear or the interpretations provided by claim reviews.

Beyond ClaimReview, the Claim type can be associated with related creative works - for example a ScholaryArticle or Question might be about some Claim.

At this time, Schema.org does not define any types of relationship between claims. This is a natural area for future exploration.</rdfs:comment>
    <rdfs:label>schema:Claim</rdfs:label>
  </rdf:Description>
  <rdf:Description rdf:about="http://schema.org/runtime">
    <rdf:type rdf:resource="http://www.w3.org/2002/07/owl#DatatypeProperty"/>
    <rdfs:comment>Runtime platform or script interpreter dependencies (example: Java v1, Python 2.3, .NET Framework 3.0).</rdfs:comment>
    <rdfs:label>schema:runtime</rdfs:label>
  </rdf:Description>
  <rdf:Description rdf:nodeID="Nd9329b165269419fa6686c17f8fe8262">
    <rdf:first rdf:resource="https://w3id.org/EVI#Software"/>
    <rdf:rest rdf:resource="http://www.w3.org/1999/02/22-rdf-syntax-ns#nil"/>
  </rdf:Description>
  <rdf:Description rdf:about="http://schema.org/fileFormat">
    <rdf:type rdf:resource="http://www.w3.org/2002/07/owl#DatatypeProperty"/>
    <rdfs:domain rdf:nodeID="Nb68e12d6e59346089a39c0711c1b6052"/>
    <rdfs:range rdf:resource="http://www.w3.org/2001/XMLSchema#string"/>
    <rdfs:comment>Media type, typically MIME format (see IANA site) of the content e.g. application/zip of a SoftwareApplication binary. In cases where a CreativeWork has several media type representations, 'encoding' can be used to indicate each MediaObject alongside particular fileFormat information. Unregistered or niche file formats can be indicated instead via the most appropriate URL, e.g. defining Web page or a Wikipedia entry.</rdfs:comment>
    <rdfs:label>schema:fileFormat</rdfs:label>
  </rdf:Description>
  <rdf:Description rdf:about="https://w3id.org/EVI#describedBy">
    <rdf:type rdf:resource="http://www.w3.org/2002/07/owl#ObjectProperty"/>
    <owl:inverseOf rdf:resource="https://w3id.org/EVI#describes"/>
    <rdfs:comment>Reverse of describes property.</rdfs:comment>
    <rdfs:label>describedBy</rdfs:label>
  </rdf:Description>
  <rdf:Description rdf:about="http://schema.org/dateCreated">
    <rdf:type rdf:resource="http://www.w3.org/2002/07/owl#DatatypeProperty"/>
    <rdfs:domain rdf:resource="https://w3id.org/EVI#Dataset"/>
    <rdfs:range rdf:resource="http://www.w3.org/2001/XMLSchema#dateTime"/>
    <rdfs:comment>Date when the item was created.</rdfs:comment>
    <rdfs:label>schema:dateCreated</rdfs:label>
  </rdf:Description>
  <rdf:Description rdf:nodeID="Nba3cc71b22eb418c8b03f631e364a8d4">
    <rdf:type rdf:resource="http://www.w3.org/2002/07/owl#Class"/>
    <owl:unionOf rdf:nodeID="N30ab2c1a589242efaa464bbd4a9d22f5"/>
  </rdf:Description>
  <rdf:Description rdf:about="https://w3id.org/EVI#Schema">
    <rdf:type rdf:resource="http://www.w3.org/2002/07/owl#Class"/>
    <rdfs:subClassOf rdf:resource="https://w3id.org/EVI#Dataset"/>
    <rdfs:comment>A semi-structured interpretation of instances of DigitalObjects that can help comprehend the content.</rdfs:comment>
    <rdfs:label>Schema</rdfs:label>
  </rdf:Description>
  <rdf:Description rdf:nodeID="N8f59881000c34ea888a66d16e3fcc7a7">
    <rdf:first rdf:resource="https://w3id.org/EVI#Dataset"/>
    <rdf:rest rdf:nodeID="N7184b94320474f6797b6a0a8eb8dda84"/>
  </rdf:Description>
  <rdf:Description rdf:about="https://w3id.org/EVI#challenges">
    <rdf:type rdf:resource="http://www.w3.org/2002/07/owl#ObjectProperty"/>
    <rdfs:domain rdf:resource="https://w3id.org/EVI#DigitalObject"/>
    <rdfs:range rdf:resource="https://w3id.org/EVI#DigitalObject"/>
    <rdfs:comment>The challenges property is entailed by property chain rule when a DigitalObject A either directly challenges another DigitalObject B, or indirectlyChallenges B by challenging a DigitalObject which supports it.</rdfs:comment>
    <rdfs:label>challenges</rdfs:label>
  </rdf:Description>
  <rdf:Description rdf:about="https://w3id.org/EVI#datasetUsedBy">
    <rdf:type rdf:resource="http://www.w3.org/2002/07/owl#ObjectProperty"/>
    <rdfs:subPropertyOf rdf:resource="https://w3id.org/EVI#usedBy"/>
    <owl:inverseOf rdf:resource="https://w3id.org/EVI#usedDataset"/>
    <rdfs:comment>Reverse of usedDataset property.</rdfs:comment>
    <rdfs:label>datasetUsedBy</rdfs:label>
  </rdf:Description>
  <rdf:Description rdf:nodeID="N8162949e877349c5bd155cb373771e67">
    <rdf:first rdf:resource="https://w3id.org/EVI#Dataset"/>
    <rdf:rest rdf:nodeID="Nd9329b165269419fa6686c17f8fe8262"/>
  </rdf:Description>
  <rdf:Description rdf:about="https://w3id.org/EVI#softwareUsedBy">
    <rdf:type rdf:resource="http://www.w3.org/2002/07/owl#ObjectProperty"/>
    <rdfs:subPropertyOf rdf:resource="https://w3id.org/EVI#usedBy"/>
    <owl:inverseOf rdf:resource="https://w3id.org/EVI#usedSoftware"/>
    <rdfs:comment>Reverse of usedSoftware property.</rdfs:comment>
    <rdfs:label>softwareUsedBy</rdfs:label>
  </rdf:Description>
  <rdf:Description rdf:about="https://w3id.org/EVI#intendedUseCase">
    <rdf:type rdf:resource="http://www.w3.org/2002/07/owl#DatatypeProperty"/>
    <rdfs:domain rdf:resource="https://w3id.org/EVI#MLModel"/>
    <rdfs:range rdf:resource="http://www.w3.org/2001/XMLSchema#string"/>
    <rdfs:comment>The context in which this model is intended to be used.</rdfs:comment>
    <rdfs:label>intendedUseCase</rdfs:label>
  </rdf:Description>
  <rdf:Description rdf:nodeID="N5c9c66fc760d4252ad7a42ce375a8b4e">
    <rdf:type rdf:resource="http://www.w3.org/2002/07/owl#Class"/>
    <owl:unionOf rdf:nodeID="N5301cd9a878d4955a4aeb3665dd0063a"/>
  </rdf:Description>
  <rdf:Description rdf:about="https://w3id.org/EVI#usedBy">
    <rdf:type rdf:resource="http://www.w3.org/2002/07/owl#ObjectProperty"/>
    <rdfs:subPropertyOf rdf:resource="https://w3id.org/EVI#directlySupports"/>
    <rdfs:comment>Reverse of used property.</rdfs:comment>
    <rdfs:label>usedBy</rdfs:label>
  </rdf:Description>
  <rdf:Description rdf:about="https://w3id.org/EVI#packagedBy">
    <rdf:type rdf:resource="http://www.w3.org/2002/07/owl#ObjectProperty"/>
    <owl:inverseOf rdf:resource="https://w3id.org/EVI#packages"/>
    <rdfs:comment>Reverse of packages property.</rdfs:comment>
    <rdfs:label>packagedBy</rdfs:label>
  </rdf:Description>
  <rdf:Description rdf:about="http://schema.org/dateModified">
    <rdf:type rdf:resource="http://www.w3.org/2002/07/owl#DatatypeProperty"/>
    <rdfs:domain rdf:nodeID="N1a0acc0547f2406aa0bf383c1955b46f"/>
    <rdfs:range rdf:resource="http://www.w3.org/2001/XMLSchema#dateTime"/>
    <rdfs:comment>The date when the item was modifed last.</rdfs:comment>
    <rdfs:label>schema:dateModified</rdfs:label>
  </rdf:Description>
  <rdf:Description rdf:about="http://schema.org/title">
    <rdf:type rdf:resource="http://www.w3.org/2002/07/owl#DatatypeProperty"/>
    <rdfs:range rdf:resource="http://www.w3.org/2001/XMLSchema#string"/>
    <rdfs:comment>The title of a Thing.</rdfs:comment>
    <rdfs:label>schema:title</rdfs:label>
  </rdf:Description>
  <rdf:Description rdf:about="https://w3id.org/EVI#containedBy">
    <rdf:type rdf:resource="http://www.w3.org/2002/07/owl#ObjectProperty"/>
    <owl:inverseOf rdf:resource="https://w3id.org/EVI#contains"/>
    <rdfs:comment>Reverse of contains property.</rdfs:comment>
    <rdfs:label>containedBy</rdfs:label>
  </rdf:Description>
  <rdf:Description rdf:about="https://w3id.org/EVI#DigitalContent">
    <rdf:type rdf:resource="http://www.w3.org/2002/07/owl#Class"/>
    <rdfs:label>DigitalContent</rdfs:label>
  </rdf:Description>
  <rdf:Description rdf:nodeID="N666773303e1446038816e54e3e21f79c">
    <rdf:first rdf:resource="https://w3id.org/EVI#Software"/>
    <rdf:rest rdf:resource="http://www.w3.org/1999/02/22-rdf-syntax-ns#nil"/>
  </rdf:Description>
  <rdf:Description rdf:about="https://w3id.org/EVI#derivedFrom">
    <rdf:type rdf:resource="http://www.w3.org/2002/07/owl#ObjectProperty"/>
    <rdfs:subPropertyOf rdf:resource="https://w3id.org/EVI#directlySupportedBy"/>
    <owl:inverseOf rdf:resource="https://w3id.org/EVI#derivedTo"/>
    <rdfs:domain rdf:resource="https://www.w3.org/ns/prov#Entity"/>
    <rdfs:range rdf:resource="https://www.w3.org/ns/prov#Entity"/>
    <rdfs:comment>A derivation is a transformation of a prov:Entity into another, an update of a prov:Entity resulting in a new one, or the construction of a new prov:Entity based on a pre-existing prov:Entity.</rdfs:comment>
    <rdfs:label>derivedFrom</rdfs:label>
  </rdf:Description>
  <rdf:Description rdf:about="https://w3id.org/EVI#framework">
    <rdf:type rdf:resource="http://www.w3.org/2002/07/owl#DatatypeProperty"/>
    <rdfs:domain rdf:resource="https://w3id.org/EVI#MLModel"/>
    <rdfs:range rdf:resource="http://www.w3.org/2001/XMLSchema#string"/>
    <rdfs:comment>The machine learning framework used to create the model (e.g., PyTorch, TensorFlow).</rdfs:comment>
    <rdfs:label>framework</rdfs:label>
  </rdf:Description>
  <rdf:Description rdf:about="https://www.w3.org/ns/prov#Entity">
    <rdf:type rdf:resource="http://www.w3.org/2002/07/owl#Class"/>
    <rdfs:comment>An Entity is a physical, digital, conceptual, or other kind of thing with some fixed aspects.</rdfs:comment>
    <rdfs:label>prov:Entity</rdfs:label>
  </rdf:Description>
  <rdf:Description rdf:about="https://w3id.org/EVI#associatedWith">
    <rdf:type rdf:resource="http://www.w3.org/2002/07/owl#ObjectProperty"/>
    <rdfs:subPropertyOf rdf:resource="https://w3id.org/EVI#directlySupportedBy"/>
    <rdfs:domain rdf:resource="https://www.w3.org/ns/prov#Activity"/>
    <rdfs:range rdf:resource="https://www.w3.org/ns/prov#Agent"/>
    <rdfs:comment>A prov:Agent that has some responsibility for the occurrence of this prov:Activity is associatedWith the prov:Activity.</rdfs:comment>
    <rdfs:label>associatedWith</rdfs:label>
  </rdf:Description>
  <rdf:Description rdf:about="https://w3id.org/EVI#Article">
    <rdf:type rdf:resource="http://www.w3.org/2002/07/owl#Class"/>
    <rdfs:subClassOf rdf:resource="https://w3id.org/EVI#DigitalObject"/>
    <rdfs:comment>An Article is a (typically compound) textual document conveying a set of Claims and other DigitalObjects. Among these, an Article in EVI always conveys an assertion of its authorship in the form of a bibliographic self-reference.</rdfs:comment>
    <rdfs:label>Article</rdfs:label>
  </rdf:Description>
  <rdf:Description rdf:about="http://schema.org/description">
    <rdf:type rdf:resource="http://www.w3.org/2002/07/owl#DatatypeProperty"/>
    <rdfs:domain rdf:resource="http://www.w3.org/2002/07/owl#Thing"/>
    <rdfs:range rdf:resource="http://www.w3.org/2001/XMLSchema#string"/>
    <rdfs:comment>A description of the item.</rdfs:comment>
    <rdfs:label>schema:description</rdfs:label>
  </rdf:Description>
  <rdf:Description rdf:about="https://www.w3.org/ns/prov#Agent">
    <rdf:type rdf:resource="http://www.w3.org/2002/07/owl#Class"/>
    <rdfs:subClassOf rdf:resource="https://www.w3.org/ns/prov#Entity"/>
    <rdfs:comment>An Agent is an autonomous Entity. Persons and Organizations are Agents in EVI. Agents may be associatedWith Activities, and Entities may be attributedTo Agents.</rdfs:comment>
    <rdfs:label>prov:Agent</rdfs:label>
  </rdf:Description>
  <rdf:Description rdf:about="https://w3id.org/EVI#directlyChallengedBy">
    <rdf:type rdf:resource="http://www.w3.org/2002/07/owl#ObjectProperty"/>
    <rdfs:subPropertyOf rdf:resource="https://w3id.org/EVI#challengedBy"/>
    <owl:inverseOf rdf:resource="https://w3id.org/EVI#directlyChallenges"/>
    <rdfs:comment>Reverse of directlyChallenges property.</rdfs:comment>
    <rdfs:label>directlyChallengedBy</rdfs:label>
  </rdf:Description>
  <rdf:Description rdf:about="https://w3id.org/EVI#DigitalObject">
    <rdf:type rdf:resource="http://www.w3.org/2002/07/owl#Class"/>
    <rdfs:subClassOf rdf:resource="https://www.w3.org/ns/prov#Entity"/>
    <rdfs:comment>A DigitalObject is an Entity which represents another Entity. DigitalObjects are always attributedTo an Agent, their creator, contributor, influencer or to an Activity they were generatedBy.</rdfs:comment>
    <rdfs:label>DigitalObject</rdfs:label>
  </rdf:Description>
  <rdf:Description rdf:nodeID="Nb3b2a52811b1478d8a737df63710616d">
    <rdf:first rdf:resource="https://w3id.org/EVI#Dataset"/>
    <rdf:rest rdf:nodeID="Nddeb8932f5be4be1b2be7c3b08c3cd83"/>
  </rdf:Description>
  <rdf:Description rdf:about="http://schema.org/author">
    <rdf:type rdf:resource="http://www.w3.org/2002/07/owl#DatatypeProperty"/>
    <rdfs:range rdf:resource="http://www.w3.org/2001/XMLSchema#string"/>
    <rdfs:comment>The author of the content.</rdfs:comment>
    <rdfs:label>schema:author</rdfs:label>
  </rdf:Description>
  <rdf:Description rdf:about="https://w3id.org/EVI#hasDistribution">
    <rdf:type rdf:resource="http://www.w3.org/2002/07/owl#ObjectProperty"/>
    <rdfs:domain rdf:resource="https://w3id.org/EVI#DigitalObject"/>
    <rdfs:range rdf:resource="https://w3id.org/EVI#Distribution"/>
    <rdfs:comment>Used to represent different forms of a DigitalObject. An image may be distributed as a JPEG, PNG, or SVG.</rdfs:comment>
    <rdfs:label>hasDistribution</rdfs:label>
  </rdf:Description>
  <rdf:Description rdf:about="https://w3id.org/EVI#serviceUsedBy">
    <rdf:type rdf:resource="http://www.w3.org/2002/07/owl#ObjectProperty"/>
    <rdfs:subPropertyOf rdf:resource="https://w3id.org/EVI#usedBy"/>
    <owl:inverseOf rdf:resource="https://w3id.org/EVI#usedService"/>
    <rdfs:comment>Reverse of usedService property.</rdfs:comment>
    <rdfs:label>serviceUsedBy</rdfs:label>
  </rdf:Description>
  <rdf:Description rdf:about="http://schema.org/version">
    <rdf:type rdf:resource="http://www.w3.org/2002/07/owl#DatatypeProperty"/>
    <rdfs:range rdf:resource="http://www.w3.org/2001/XMLSchema#string"/>
    <rdfs:comment>The version of the DigitalObject.</rdfs:comment>
    <rdfs:label>schema:version</rdfs:label>
  </rdf:Description>
  <rdf:Description rdf:about="https://w3id.org/EVI#represents">
    <rdf:type rdf:resource="http://www.w3.org/2002/07/owl#ObjectProperty"/>
    <rdfs:domain rdf:resource="https://w3id.org/EVI#DigitalObject"/>
    <rdfs:range rdf:resource="https://www.w3.org/ns/prov#Entity"/>
    <rdfs:comment>A DigitalObject represents an Entity or any of its features or feature sets.</rdfs:comment>
    <rdfs:label>represents</rdfs:label>
  </rdf:Description>
  <rdf:Description rdf:nodeID="N2a95c47191824e0a8d53674395752438">
    <rdf:first rdf:resource="https://w3id.org/EVI#directlyChallenges"/>
    <rdf:rest rdf:nodeID="N2b0e6260a6d14db3b35eca0c82c66508"/>
  </rdf:Description>
  <rdf:Description rdf:about="https://w3id.org/EVI#ROCrate">
    <rdf:type rdf:resource="http://www.w3.org/2002/07/owl#Class"/>
    <rdfs:subClassOf rdf:resource="https://w3id.org/EVI#Package"/>
    <rdfs:comment>An approach to packaging research data with their metadata.</rdfs:comment>
    <rdfs:label>ROCrate</rdfs:label>
  </rdf:Description>
  <rdf:Description rdf:nodeID="N69e9bc263b7a492da24c709fe879c29c">
    <rdf:type rdf:resource="http://www.w3.org/2002/07/owl#Class"/>
    <owl:unionOf rdf:nodeID="Nc438f93256cc4b82ba6c3f9b7ef21214"/>
  </rdf:Description>
  <rdf:Description rdf:nodeID="Na2a23265f6ca456b8af943cdb0ed1672">
    <rdf:type rdf:resource="http://www.w3.org/2002/07/owl#Class"/>
    <owl:unionOf rdf:nodeID="N37ffb79d9a2d409c92e86008f6519fed"/>
  </rdf:Description>
  <rdf:Description rdf:nodeID="Neb884f4e80674c5bb4037a54ab34d6bd">
    <rdf:first rdf:resource="https://w3id.org/EVI#Software"/>
    <rdf:rest rdf:resource="http://www.w3.org/1999/02/22-rdf-syntax-ns#nil"/>
  </rdf:Description>
  <rdf:Description rdf:about="https://orcid.org/0000-0003-4647-3877">
    <rdf:type rdf:resource="http://www.w3.org/2002/07/owl#NamedIndividual"/>
  </rdf:Description>
  <rdf:Description rdf:about="http://purl.org/vocab/vann/preferredNamespaceUri">
    <rdf:type rdf:resource="http://www.w3.org/2002/07/owl#AnnotationProperty"/>
  </rdf:Description>
  <rdf:Description rdf:about="http://purl.org/dc/terms/license">
    <rdf:type rdf:resource="http://www.w3.org/2002/07/owl#AnnotationProperty"/>
  </rdf:Description>
  <rdf:Description rdf:about="http://schema.org/endTime">
    <rdf:type rdf:resource="http://www.w3.org/2002/07/owl#DatatypeProperty"/>
    <rdfs:domain rdf:resource="https://w3id.org/EVI#Computation"/>
    <rdfs:range rdf:resource="http://www.w3.org/2001/XMLSchema#dateTime"/>
    <rdfs:comment>The endTime of something. For a reserved event or service (e.g. FoodEstablishmentReservation), the time that it is expected to end. For actions that span a period of time, when the action was performed. e.g. John wrote a book from January to December. For media, including audio and video, it's the time offset of the end of a clip within a larger file.

Note that Event uses startDate/endDate instead of startTime/endTime, even when describing dates with times. This situation may be clarified in future revisions.</rdfs:comment>
    <rdfs:label>schema:endTime</rdfs:label>
  </rdf:Description>
  <rdf:Description rdf:nodeID="N656d1f893b73479faf005b0166bb7695">
    <rdf:type rdf:resource="http://www.w3.org/2002/07/owl#Class"/>
    <owl:unionOf rdf:nodeID="N889afee0109c4667a285af07340dad3c"/>
  </rdf:Description>
  <rdf:Description rdf:nodeID="Nc438f93256cc4b82ba6c3f9b7ef21214">
    <rdf:first rdf:resource="https://w3id.org/EVI#Dataset"/>
    <rdf:rest rdf:nodeID="Neb884f4e80674c5bb4037a54ab34d6bd"/>
  </rdf:Description>
  <rdf:Description rdf:about="http://schema.org/Person">
    <rdf:type rdf:resource="http://www.w3.org/2002/07/owl#Class"/>
    <owl:equivalentClass rdf:resource="https://www.w3.org/ns/prov#Person"/>
    <rdfs:subClassOf rdf:resource="https://www.w3.org/ns/prov#Agent"/>
    <rdfs:comment>A person (alive, dead, undead, or fictional).</rdfs:comment>
    <rdfs:label>schema:Person</rdfs:label>
  </rdf:Description>
  <rdf:Description rdf:nodeID="N17971ccadfe0494485b7dae2ed371e61">
    <rdf:first rdf:resource="http://www.w3.org/2001/XMLSchema#anyURI"/>
    <rdf:rest rdf:nodeID="Nbaeeda7fc8d44f68bd57717aefd165a1"/>
  </rdf:Description>
  <rdf:Description rdf:nodeID="N7ac8284c91ac4bffa957425012b54369">
    <rdf:first rdf:resource="https://w3id.org/EVI#Software"/>
    <rdf:rest rdf:resource="http://www.w3.org/1999/02/22-rdf-syntax-ns#nil"/>
  </rdf:Description>
  <rdf:Description rdf:nodeID="N640fb088466a41e683040b8b91eceb73">
    <rdf:type rdf:resource="http://www.w3.org/2000/01/rdf-schema#Datatype"/>
    <owl:unionOf rdf:nodeID="N17971ccadfe0494485b7dae2ed371e61"/>
  </rdf:Description>
  <rdf:Description rdf:nodeID="N2419b5b626154ae6b71f75b474dc6817">
    <rdf:type rdf:resource="http://www.w3.org/2000/01/rdf-schema#Datatype"/>
    <owl:unionOf rdf:nodeID="Nce33bcf0eca3438ca339c18cbafc8472"/>
  </rdf:Description>
  <rdf:Description rdf:about="https://w3id.org/EVI#usedSoftware">
    <rdf:type rdf:resource="http://www.w3.org/2002/07/owl#ObjectProperty"/>
    <rdfs:subPropertyOf rdf:resource="https://w3id.org/EVI#used"/>
    <rdfs:domain rdf:resource="https://w3id.org/EVI#Computation"/>
    <rdfs:range rdf:resource="https://w3id.org/EVI#Software"/>
    <rdfs:comment>The property usedSoftware is a subproperty of used where domain is Computation and range is Software.</rdfs:comment>
    <rdfs:label>usedSoftware</rdfs:label>
  </rdf:Description>
  <rdf:Description rdf:about="https://w3id.org/EVI#generatedBy">
    <rdf:type rdf:resource="http://www.w3.org/2002/07/owl#ObjectProperty"/>
    <rdfs:subPropertyOf rdf:resource="https://w3id.org/EVI#directlySupportedBy"/>
    <rdfs:domain rdf:resource="https://www.w3.org/ns/prov#Entity"/>
    <rdfs:range rdf:resource="https://www.w3.org/ns/prov#Activity"/>
    <rdfs:comment>Generation is the completion of production of a new prov:Entity by a prov:Activity. This entity did not exist before generation and becomes available for usage after this generation.</rdfs:comment>
    <rdfs:label>generatedBy</rdfs:label>
  </rdf:Description>
  <rdf:Description rdf:about="http://schema.org/contentSize">
    <rdf:type rdf:resource="http://www.w3.org/2002/07/owl#DatatypeProperty"/>
    <rdfs:domain rdf:nodeID="Na2a23265f6ca456b8af943cdb0ed1672"/>
    <rdfs:range rdf:resource="http://www.w3.org/2001/XMLSchema#long"/>
    <rdfs:comment>File size in (tera/giga/mega/kilo) bytes.</rdfs:comment>
    <rdfs:label>schema:contentSize</rdfs:label>
  </rdf:Description>
  <rdf:Description rdf:about="http://purl.org/dc/terms/description">
    <rdf:type rdf:resource="http://www.w3.org/2002/07/owl#AnnotationProperty"/>
  </rdf:Description>
  <rdf:Description rdf:about="http://purl.org/dc/terms/modified">
    <rdf:type rdf:resource="http://www.w3.org/2002/07/owl#AnnotationProperty"/>
  </rdf:Description>
  <rdf:Description rdf:nodeID="N4eddae4666c74b9c97a49ca0b2b38b20">
    <rdf:first rdf:resource="https://w3id.org/EVI#Dataset"/>
    <rdf:rest rdf:nodeID="Nc08456ff66e7487d962bee0ad288ebd6"/>
  </rdf:Description>
  <rdf:Description rdf:nodeID="N9fe00874ee1140099f4ff5d1a8a06bd2">
    <rdf:first rdf:resource="https://w3id.org/EVI#Software"/>
    <rdf:rest rdf:resource="http://www.w3.org/1999/02/22-rdf-syntax-ns#nil"/>
  </rdf:Description>
  <rdf:Description rdf:nodeID="N7184b94320474f6797b6a0a8eb8dda84">
    <rdf:first rdf:resource="https://w3id.org/EVI#Software"/>
    <rdf:rest rdf:resource="http://www.w3.org/1999/02/22-rdf-syntax-ns#nil"/>
  </rdf:Description>
  <rdf:Description rdf:nodeID="Nf6baaac2ae19410d826477c86e93aa22">
    <rdf:first rdf:resource="https://w3id.org/EVI#Software"/>
    <rdf:rest rdf:resource="http://www.w3.org/1999/02/22-rdf-syntax-ns#nil"/>
  </rdf:Description>
  <rdf:Description rdf:nodeID="Nee56742a1c524eefba7f015572ab5965">
    <rdf:type rdf:resource="http://www.w3.org/2002/07/owl#Class"/>
    <owl:unionOf rdf:nodeID="Nb6530a0fd8e448bf91e980b1094da6e8"/>
  </rdf:Description>
  <rdf:Description rdf:nodeID="Nc43f5969fcee4317bf697e29229e71d8">
    <rdf:first rdf:resource="https://w3id.org/EVI#Dataset"/>
    <rdf:rest rdf:nodeID="Nf6baaac2ae19410d826477c86e93aa22"/>
  </rdf:Description>
  <rdf:Description rdf:nodeID="N86b379137d3d4f95a9b54f23c7682f1d">
    <rdf:first rdf:resource="http://www.w3.org/2001/XMLSchema#anyURI"/>
    <rdf:rest rdf:nodeID="N4172f5b5abb849a998fabbdaea104bde"/>
  </rdf:Description>
  <rdf:Description rdf:nodeID="Nb6530a0fd8e448bf91e980b1094da6e8">
    <rdf:first rdf:resource="https://w3id.org/EVI#Dataset"/>
    <rdf:rest rdf:nodeID="N3296ec73c8a44bb2ba1818e1f59d5ee5"/>
  </rdf:Description>
  <rdf:Description rdf:nodeID="N3296ec73c8a44bb2ba1818e1f59d5ee5">
    <rdf:first rdf:resource="https://w3id.org/EVI#Software"/>
    <rdf:rest rdf:resource="http://www.w3.org/1999/02/22-rdf-syntax-ns#nil"/>
  </rdf:Description>
  <rdf:Description rdf:about="http://swrl.stanford.edu/ontologies/3.3/swrla.owl#isRuleEnabled">
    <rdf:type rdf:resource="http://www.w3.org/2002/07/owl#AnnotationProperty"/>
  </rdf:Description>
  <rdf:Description rdf:nodeID="Na341cade5df7416fa0fc8cd5e200d20a">
    <rdf:type rdf:resource="http://www.w3.org/2002/07/owl#Class"/>
    <owl:unionOf rdf:nodeID="Nd1e9f5743eed4ccea29525833a324206"/>
  </rdf:Description>
  <rdf:Description rdf:nodeID="Nb68e12d6e59346089a39c0711c1b6052">
    <rdf:type rdf:resource="http://www.w3.org/2002/07/owl#Class"/>
    <owl:unionOf rdf:nodeID="N8162949e877349c5bd155cb373771e67"/>
  </rdf:Description>
  <rdf:Description rdf:about="http://www.w3.org/2002/07/owl#versionIRI">
    <rdf:type rdf:resource="http://www.w3.org/2002/07/owl#AnnotationProperty"/>
  </rdf:Description>
  <rdf:Description rdf:nodeID="Nbaeeda7fc8d44f68bd57717aefd165a1">
    <rdf:first rdf:resource="http://www.w3.org/2001/XMLSchema#string"/>
    <rdf:rest rdf:resource="http://www.w3.org/1999/02/22-rdf-syntax-ns#nil"/>
  </rdf:Description>
  <rdf:Description rdf:nodeID="Nc08456ff66e7487d962bee0ad288ebd6">
    <rdf:first rdf:resource="https://w3id.org/EVI#Software"/>
    <rdf:rest rdf:resource="http://www.w3.org/1999/02/22-rdf-syntax-ns#nil"/>
  </rdf:Description>
  <rdf:Description rdf:nodeID="N3d13ed0d04f04c51a095f813997f2c7e">
    <rdf:first rdf:resource="http://www.w3.org/2001/XMLSchema#string"/>
    <rdf:rest rdf:resource="http://www.w3.org/1999/02/22-rdf-syntax-ns#nil"/>
  </rdf:Description>
</rdf:RDF>
